seplog/ast.v
@@ -91,21 +91,27 @@ Inductive stmt: Type :=
 | s_assign: var -> expr -> stmt
 | s_load: var -> expr -> stmt
 | s_store: var -> expr -> stmt
-| s_scope: stmt -> stmt
 | s_if: expr -> stmt -> stmt -> stmt
 | s_while: expr -> stmt -> stmt
 | s_call: var -> proc -> expr -> stmt
-| s_local: var -> expr -> stmt
 | s_return: expr -> stmt
 | s_getlock: var -> stmt
 | s_putlock: var -> stmt
 with
 
 (*
+ * variable declarations take values
+ * (everything needs to be initialized)
+ *)
+(*Inductive*) vardecl: Type :=
+| mkvardecl: var -> expr -> vardecl
+with
+
+(*
  * procs both take and produce values
  *)
 (*Inductive*) proc: Type :=
-| mkproc: type -> var -> stmt -> proc
+| mkproc: type -> var -> list vardecl -> stmt -> proc
 .
 
 
